Foundation/Modal/Kripke/Logic/Grz/Soundness.lean
@@ -1,4 +1,7 @@
 import Foundation.Modal.Kripke.AxiomGrz
+import Foundation.Modal.Hilbert.WellKnown
+import Foundation.Modal.Kripke.Logic.S4M
+import Mathlib.Order.Preorder.Finite
 
 namespace LO.Modal
 
@@ -11,24 +14,46 @@ open Hilbert.Kripke
 
 namespace Kripke
 
-protected abbrev FrameClass.trans_wcwf : FrameClass := { F | IsPreorder _ F.Rel ∧ IsWeaklyConverseWellFounded _ F.Rel }
-protected abbrev FrameClass.finite_partial_order: FrameClass := { F | F.IsFinite ∧ IsPartialOrder _ F.Rel }
+variable {F : Frame}
+
+protected class Frame.IsFiniteGrz (F : Frame) extends F.IsFinite, F.IsPartialOrder
+
+protected abbrev FrameClass.finite_Grz: FrameClass := { F | F.IsFiniteGrz }
+
+instance : whitepoint.IsAntisymmetric := ⟨by tauto⟩
+instance : whitepoint.IsFiniteGrz where
+
+instance [F.IsFinite] [F.IsPartialOrder] : F.SatisfiesMcKinseyCondition where
+  mckinsey := by
+    intro x;
+    obtain ⟨y, _, Rxy, hy₃⟩ :=  @Finite.exists_le_maximal _ {
+      le := F,
+      le_refl := fun a ↦ Frame.refl,
+      le_trans := fun x y z ↦ Frame.trans
+    } _ (λ y => x ≺ y) x Frame.refl;
+    use y;
+    constructor;
+    . tauto;
+    . intro z Ryz;
+      apply F.antisymm;
+      . assumption;
+      . exact @hy₃ z (F.trans Rxy Ryz) Ryz;
+instance [F.IsFiniteGrz] : F.IsS4M where
 
 end Kripke
 
 
 namespace Hilbert.Grz.Kripke
 
-instance finite_sound : Sound (Hilbert.Grz) FrameClass.finite_partial_order := instSound_of_validates_axioms $ by
+instance finite_sound : Sound (Hilbert.Grz) FrameClass.finite_Grz := instSound_of_validates_axioms $ by
   apply FrameClass.Validates.withAxiomK;
   rintro F ⟨_, _⟩ _ rfl;
   exact validate_AxiomGrz_of_refl_trans_wcwf;
 
 instance consistent : Entailment.Consistent (Hilbert.Grz) :=
-  consistent_of_sound_frameclass FrameClass.finite_partial_order $ by
+  consistent_of_sound_frameclass FrameClass.finite_Grz $ by
     use whitepoint;
-    apply Set.mem_setOf_eq.mpr;
-    exact ⟨inferInstance, inferInstance⟩
+    constructor;
 
 end Hilbert.Grz.Kripke
 
