Foundation/Modal/Kripke/Logic/S4.lean
@@ -7,51 +7,49 @@ namespace LO.Modal
 
 open Kripke
 open Hilbert.Kripke
-open GeachConfluent
 
 
 namespace Kripke
 
-protected abbrev FrameClass.preorder : FrameClass := { F | IsPreorder _ F }
+protected abbrev Frame.IsS4 := Frame.IsPreorder
+protected class Frame.IsFiniteS4 (F : Frame) extends F.IsFinite, F.IsS4
 
-protected abbrev FrameClass.finite_preorder: FrameClass := { F | Finite F.World ∧ IsPreorder _ F.Rel }
+protected abbrev FrameClass.S4 : FrameClass := { F | F.IsS4 }
+protected abbrev FrameClass.finite_S4 : FrameClass := { F | F.IsFiniteS4 }
 
 end Kripke
 
 
 namespace Hilbert.S4.Kripke
 
-instance sound : Sound (Hilbert.S4) Kripke.FrameClass.preorder := instSound_of_validates_axioms $ by
+instance sound : Sound (Hilbert.S4) FrameClass.S4 := instSound_of_validates_axioms $ by
   apply FrameClass.Validates.withAxiomK;
   rintro F ⟨_, _⟩ _ (rfl | rfl);
   . exact validate_AxiomT_of_reflexive;
   . exact validate_AxiomFour_of_transitive;
 
-instance consistent : Entailment.Consistent (Hilbert.S4) := consistent_of_sound_frameclass Kripke.FrameClass.preorder $ by
+instance consistent : Entailment.Consistent (Hilbert.S4) := consistent_of_sound_frameclass FrameClass.S4 $ by
   use whitepoint;
   constructor;
 
-instance canonical : Canonical (Hilbert.S4) Kripke.FrameClass.preorder := ⟨by
-  apply Set.mem_setOf_eq.mpr;
-  constructor;
-⟩
+instance canonical : Canonical (Hilbert.S4) FrameClass.S4 := ⟨by constructor⟩
 
-instance complete : Complete (Hilbert.S4) Kripke.FrameClass.preorder := inferInstance
+instance complete : Complete (Hilbert.S4) FrameClass.S4 := inferInstance
 
 open finestFiltrationTransitiveClosureModel in
-instance finiteComplete : Complete (Hilbert.S4) Kripke.FrameClass.finite_preorder := ⟨by
+instance finiteComplete : Complete (Hilbert.S4) FrameClass.finite_S4 := ⟨by
   intro φ hp;
   apply Kripke.complete.complete;
-  rintro F F_preorder V x;
-  replace F_preorder := Set.mem_setOf_eq.mp F_preorder;
+  rintro F hF V x;
+  replace hF := Set.mem_setOf_eq.mp hF;
   let M : Kripke.Model := ⟨F, V⟩;
   let FM := finestFiltrationTransitiveClosureModel M φ.subformulas;
-  apply filtration FM (finestFiltrationTransitiveClosureModel.filterOf) (by subformula) |>.mpr;
+  apply filtration FM filterOf (by simp) |>.mpr;
   apply hp;
-  refine ⟨?_, ?_⟩;
-  . apply FilterEqvQuotient.finite;
-    simp;
-  . exact finestFiltrationTransitiveClosureModel.isPreorder;
+  refine {
+    world_finite := by apply FilterEqvQuotient.finite $ by simp;
+    refl := finestFiltrationTransitiveClosureModel.isReflexive.refl
+  }
 ⟩
 
 end Hilbert.S4.Kripke
@@ -62,13 +60,13 @@ open Formula
 open Entailment
 open Kripke
 
-lemma S4.Kripke.preorder : Logic.S4 = FrameClass.preorder.logic := eq_hilbert_logic_frameClass_logic
+lemma S4.Kripke.preorder : Logic.S4 = FrameClass.S4.logic := eq_hilbert_logic_frameClass_logic
 
 @[simp]
 theorem S4.proper_extension_of_KT : Logic.KT ⊂ Logic.S4 := by
   constructor;
   . exact Hilbert.weakerThan_of_dominate_axioms (by simp [axiomK!, axiomT!]) |>.subset;
-  . suffices ∃ φ, Hilbert.S4 ⊢! φ ∧ ¬Kripke.FrameClass.refl ⊧ φ by
+  . suffices ∃ φ, Hilbert.S4 ⊢! φ ∧ ¬FrameClass.KT ⊧ φ by
       rw [KT.Kripke.refl];
       tauto;
     use Axioms.Four (.atom 0);
@@ -81,7 +79,7 @@ theorem S4.proper_extension_of_KT : Logic.KT ⊂ Logic.S4 := by
         ⟩;
       use M, 0;
       constructor;
-      . refine ⟨by omega⟩;
+      . exact { refl := by omega };
       . suffices (∀ (y : M.World), (0 : M.World) ≺ y → y = 0 ∨ y = 1) ∧ ∃ x, (0 : M.World) ≺ x ∧ ∃ y, x ≺ y ∧ y ≠ 0 ∧ y ≠ 1 by
           simpa [M, Semantics.Realize, Satisfies];
         constructor;
@@ -100,7 +98,7 @@ theorem S4.proper_extension_of_KT : Logic.KT ⊂ Logic.S4 := by
 theorem S4.proper_extension_of_KD4 : Logic.KD4 ⊂ Logic.S4 := by
   constructor;
   . exact Hilbert.weakerThan_of_dominate_axioms (by simp) |>.subset;
-  . suffices ∃ φ, Hilbert.S4 ⊢! φ ∧ ¬FrameClass.serial_trans ⊧ φ by
+  . suffices ∃ φ, Hilbert.S4 ⊢! φ ∧ ¬FrameClass.KD4 ⊧ φ by
       rw [KD4.Kripke.serial_trans];
       tauto;
     use Axioms.T (.atom 0);
@@ -109,7 +107,10 @@ theorem S4.proper_extension_of_KD4 : Logic.KD4 ⊂ Logic.S4 := by
     . apply Kripke.not_validOnFrameClass_of_exists_model_world;
       use ⟨⟨Fin 3, λ _ y => y = 1⟩, (λ w _ => w = 1)⟩, 0;
       constructor;
-      . refine ⟨⟨by tauto⟩, ⟨by omega⟩⟩;
+      . refine {
+          serial := by simp [Serial],
+          trans := by simp
+        };
       . simp [Semantics.Realize, Satisfies];
 
 @[simp]
