Foundation/Modal/Kripke/Logic/S4M.lean
@@ -7,32 +7,36 @@ namespace LO.Modal
 
 open Kripke
 open Hilbert.Kripke
-open GeachConfluent
 
-abbrev Kripke.FrameClass.preorder_mckinsey : FrameClass := { F | IsPreorder _ F ∧ SatisfiesMcKinseyCondition _ F }
+namespace Kripke
+
+variable {F : Kripke.Frame}
+
+class Frame.IsS4M (F : Kripke.Frame) extends F.IsReflexive, F.IsTransitive, F.SatisfiesMcKinseyCondition where
+
+abbrev FrameClass.S4M : FrameClass := { F | F.IsS4M }
+
+end Kripke
+
+
 
 namespace Hilbert.S4M
 
-instance Kripke.sound : Sound (Hilbert.S4M) (Kripke.FrameClass.preorder_mckinsey) := instSound_of_validates_axioms $ by
+instance Kripke.sound : Sound (Hilbert.S4M) FrameClass.S4M := instSound_of_validates_axioms $ by
   apply FrameClass.Validates.withAxiomK;
   rintro F ⟨_, _⟩ _ (rfl | rfl | rfl);
   . exact validate_AxiomT_of_reflexive;
   . exact validate_AxiomFour_of_transitive;
   . exact validate_axiomM_of_satisfiesMcKinseyCondition;
 
-instance Kripke.consistent : Entailment.Consistent (Hilbert.S4M) := consistent_of_sound_frameclass Kripke.FrameClass.preorder_mckinsey $ by
+instance Kripke.consistent : Entailment.Consistent (Hilbert.S4M) := consistent_of_sound_frameclass FrameClass.S4M $ by
   use whitepoint;
   apply Set.mem_setOf_eq.mpr;
-  constructor <;> infer_instance;
+  constructor
 
-instance Kripke.canonical : Canonical (Hilbert.S4M) Kripke.FrameClass.preorder_mckinsey := ⟨by
-  apply Set.mem_setOf_eq.mpr;
-  constructor;
-  . infer_instance;
-  . infer_instance;
-⟩
+instance Kripke.canonical : Canonical (Hilbert.S4M) FrameClass.S4M := ⟨by constructor⟩
 
-instance Kripke.complete : Complete (Hilbert.S4M) Kripke.FrameClass.preorder_mckinsey := inferInstance
+instance Kripke.complete : Complete (Hilbert.S4M) FrameClass.S4M := inferInstance
 
 end Hilbert.S4M
 
@@ -42,13 +46,13 @@ open Formula
 open Entailment
 open Kripke
 
-lemma S4M.Kripke.preorder_mckinsey : Logic.S4M = FrameClass.preorder_mckinsey.logic := eq_hilbert_logic_frameClass_logic
+lemma S4M.Kripke.preorder_mckinsey : Logic.S4M = FrameClass.S4M.logic := eq_hilbert_logic_frameClass_logic
 
 @[simp]
 theorem S4M.proper_extension_of_S4 : Logic.S4 ⊂ Logic.S4M := by
   constructor;
   . exact Hilbert.weakerThan_of_dominate_axioms (by simp) |>.subset;
-  . suffices ∃ φ, Hilbert.S4M ⊢! φ ∧ ¬FrameClass.preorder ⊧ φ by
+  . suffices ∃ φ, Hilbert.S4M ⊢! φ ∧ ¬FrameClass.S4 ⊧ φ by
       rw [S4.Kripke.preorder];
       tauto;
     use (Axioms.M (.atom 0));
@@ -58,8 +62,10 @@ theorem S4M.proper_extension_of_S4 : Logic.S4 ⊂ Logic.S4M := by
       let M : Model := ⟨⟨Fin 2, λ x y => True⟩, λ w _ => w = 0⟩;
       use M, 0;
       constructor;
-      . apply isPreorder_iff _ _ |>.mpr;
-        refine ⟨⟨?_⟩, ⟨?_⟩⟩ <;> simp [M];
+      . refine {
+          refl := by tauto;
+          trans := by tauto;
+        }
       . suffices ∃ x, x ≠ (0 : M.World) by simpa [M, Transitive, Reflexive, Semantics.Realize, Satisfies];
         use 1;
         trivial;
@@ -68,7 +74,7 @@ theorem S4M.proper_extension_of_S4 : Logic.S4 ⊂ Logic.S4M := by
 theorem S4M.proper_extension_of_K4M : Logic.K4M ⊂ Logic.S4M := by
   constructor;
   . exact Hilbert.weakerThan_of_dominate_axioms (by simp) |>.subset;
-  . suffices ∃ φ, Hilbert.S4M ⊢! φ ∧ ¬FrameClass.trans_mckinsey ⊧ φ by
+  . suffices ∃ φ, Hilbert.S4M ⊢! φ ∧ ¬FrameClass.K4M ⊧ φ by
       rw [K4M.Kripke.trans_mckinsey];
       tauto;
     use (Axioms.T (.atom 0));
@@ -78,9 +84,13 @@ theorem S4M.proper_extension_of_K4M : Logic.K4M ⊂ Logic.S4M := by
       let M : Model := ⟨⟨Fin 2, λ x y => y = 1⟩, λ w _ => w = 1⟩;
       use M, 0;
       constructor;
-      . refine ⟨⟨?_⟩, ⟨?_⟩⟩;
-        . omega;
-        . simp [M, McKinseyCondition];
+      . exact {
+          trans := by omega;
+          mckinsey := by
+            simp only [Fin.isValue, forall_eq, and_self, M];
+            intro;
+            use 1;
+        }
       . simp [Semantics.Realize, Satisfies, M];
 
 end Logic
