Foundation/Modal/Boxdot/Basic.lean
@@ -1,5 +1,6 @@
 import Foundation.Modal.Hilbert.Basic
 import Foundation.Modal.Kripke.Closure
+import Foundation.Modal.Kripke.Irreflexivize
 
 namespace LO.Modal
 
@@ -71,7 +72,7 @@ lemma iff_frame_boxdot_reflexive_closure : (F ⊧ (φᵇ)) ↔ ((F^=) ⊧ φ) :=
   . intro h V x; apply iff_boxdot_reflexive_closure.mp; exact h V x;
   . intro h V x; apply iff_boxdot_reflexive_closure.mpr; exact h V x;
 
-lemma iff_reflexivize_irreflexivize [IsRefl _ F] {x : F.World} {V} : (Satisfies ⟨F, V⟩ x φ) ↔ (Satisfies ⟨F^≠^=, V⟩ x φ) := by
+lemma iff_reflexivize_irreflexivize [F.IsReflexive] {x : F.World} {V} : (Satisfies ⟨F, V⟩ x φ) ↔ (Satisfies ⟨F^≠^=, V⟩ x φ) := by
   induction φ generalizing x with
   | hatom φ => rfl;
   | hfalsum => rfl;
@@ -90,7 +91,7 @@ lemma iff_reflexivize_irreflexivize [IsRefl _ F] {x : F.World} {V} : (Satisfies 
       exact h y $ by
         induction Rxy with
         | refl => apply IsRefl.refl;
-        | single h => exact h.2;
+        | single h => exact h.1;
     . intro h y Rxy;
       by_cases e : x = y;
       . subst e;
@@ -98,9 +99,9 @@ lemma iff_reflexivize_irreflexivize [IsRefl _ F] {x : F.World} {V} : (Satisfies 
         exact h x ReflGen.refl;
       . apply ihp (x := y) |>.mpr;
         exact h y $ by
-          exact ReflGen.single ⟨(by simpa), Rxy⟩;
+          exact ReflGen.single ⟨Rxy, (by simpa)⟩;
 
-lemma iff_reflexivize_irreflexivize' [IsRefl _ F] : (F ⊧ φ) ↔ ((F^≠^=) ⊧ φ) := by
+lemma iff_reflexivize_irreflexivize' [F.IsReflexive] : (F ⊧ φ) ↔ ((F^≠^=) ⊧ φ) := by
   constructor;
   . intro h V x; apply iff_reflexivize_irreflexivize.mp; exact h V x;
   . intro h V x; apply iff_reflexivize_irreflexivize.mpr; exact h V x;
